WIP: Progress on ring leader election example

theories/examples/ring_leader_election.v
@@ -1,71 +1,229 @@
 From actris.channel Require Import proofmode.
 From iris.heap_lang Require Import proofmode.
 From actris.utils Require Import contribution.
+From iris.base_logic.lib Require Import mnat.
+From iris.heap_lang.lib Require Import par assert.
 
 Definition cont := true.
 Definition elected := false.
 
+Definition abort := #() #().
+
+(** Inspired by https://en.wikipedia.org/wiki/Chang_and_Roberts_algorithm *)
+
 Definition process : val :=
   rec: "go" "id" "cl" "cr" :=
-    if: ~ (recv "cr") then
-      send "cl" #elected;; send "cl" (recv "cr");;
-      #() (* Do termination of non-leader here *)
-    else
+    if: (recv "cr") then
       let: "id'" := recv "cr" in
-      if: "id" = "id'" then send "cl" #elected;; send "cl" "id";;
-                            #() (* Do termination of leader here *)
-      else if: "id" < "id'" then send "cl" #cont;; send "cl" "id'";;
-                                 "go" "id" "cl" "cr"
+      if: "id" < "id'"          (** Case 1 *)
+      then send "cl" #cont;; send "cl" "id'";;
+           "go" "id" "cl" "cr"
+      else if: "id" = "id'"     (** Case 4 *)
+      then send "cl" #elected;; send "cl" "id";;
+           "id" (* Do termination of leader here *)
       else send "cl" #cont;; send "cl" "id";;
-           "go" "id" "cl" "cr".
+           "go" "id" "cl" "cr"
+    else
+      let: "res" := recv "cr" in
+      (* if: "id" < "res": do else ABORT *)
+      send "cl" #elected;; send "cl" "res";;
+      "res". (* Do termination of non-leader here *)
+
+Definition program : val :=
+  λ: <>,
+     let: "c1" := new_chan #() in
+     let: "c2" := new_chan #() in
+     let: "c3" := new_chan #() in
+     send (Fst "c1") #cont;; send (Fst "c1") #1;;
+     let: "res" := ( process #1 (Fst "c1") (Snd "c3")  |||
+       ( process #2 (Fst "c2") (Snd "c1") ||| process #3 (Fst "c3") (Snd "c2")) ) in
+     let: "res1" := Fst "res" in
+     let: "res2" := Fst (Snd "res") in
+     let: "res3" := Snd (Snd "res") in
+     assert: ("res1" = "res2");; assert: ("res2" = "res3");;
+     "res1".
 
 Section ring_leader_election_example.
-  Context `{!heapG Σ, chanG Σ}.
+  Context `{!heapG Σ, chanG Σ, spawnG Σ, mnatG Σ}.
 
-  Definition rle_prot_aux (rec : Z -d> iProto Σ) : Z -d> iProto Σ :=
-    λ (max_id : Z),
-      ((<! (id:Z)> MSG #id ; rec (Z.max max_id id))
+  Definition rle_prot_aux (γ : gname) (ids : gset nat) (rec : nat -d> iProto Σ)
+    : nat -d> iProto Σ :=
+    λ (max_id : nat),
+      ((<! (id:nat)> MSG #id {{ ⌜id ∈ ids⌝ ∗ mnat_own_auth γ 1 id }} ; rec id)
          <+>
-       (<!> MSG #max_id ; END))%proto.
-  Instance rle_prot_aux_contractive : Contractive rle_prot_aux.
+       (<! (q:Qp)> MSG #max_id {{ ⌜max_id ∈ ids⌝ ∗ mnat_own_auth γ q max_id }} ; END))%proto.
+  Instance rle_prot_aux_contractive γ ids : Contractive (rle_prot_aux γ ids).
   Proof. solve_proto_contractive. Qed.
-  Definition rle_prot := fixpoint rle_prot_aux.
-  Instance rle_prot_unfold max_id :
-    ProtoUnfold (rle_prot max_id) (rle_prot_aux rle_prot max_id).
-  Proof. apply proto_unfold_eq, (fixpoint_unfold rle_prot_aux). Qed.
-  
-  Lemma process_spec id cl cr :
-    {{{ cl ↣ (rle_prot id) ∗ cr ↣ iProto_dual (rle_prot id) }}}
+  Definition rle_prot γ ids := fixpoint (rle_prot_aux γ ids).
+  Instance rle_prot_unfold γ ids max_id :
+    ProtoUnfold (rle_prot γ ids max_id) (rle_prot_aux γ ids (rle_prot γ ids) max_id).
+  Proof. apply proto_unfold_eq, (fixpoint_unfold (rle_prot_aux γ ids)). Qed.
+
+  Definition rle_preprot (γ : gname) (ids : gset nat) : iProto Σ :=
+    (<!> MSG #true; <! (id:nat)> MSG #id
+                      {{ ⌜id ∈ ids⌝ ∗ mnat_own_auth γ 1 id }};
+    rle_prot γ ids id)%proto.
+
+  Lemma process_spec γ ids id max_in max_out cl cr :
+    id ∈ ids →
+    {{{ ⌜max max_in id <= max_out⌝ ∗ mnat_own_lb γ max_out ∗
+        cl ↣ (rle_prot γ ids max_out) ∗ cr ↣ iProto_dual (rle_prot γ ids max_in) }}}
       process #id cl cr
-    {{{ RET #(); True }}}.
+    {{{ res q, RET #res; ⌜id <= res⌝ ∗ ⌜res ∈ ids⌝ ∗ mnat_own_auth γ q res }}}.
   Proof.
-    iIntros (Φ) "[Hcl Hcr] HΦ".
-    iLöb as "IH" forall (id).
+    iIntros (Hin Φ) "(Hle & Hown & Hcl & Hcr) HΦ".
+    iDestruct "Hle" as %Hle.
+    iLöb as "IH" forall (max_in max_out Hle).
     wp_rec.
     wp_branch.
-    - wp_recv (id') as "_".
-      wp_pures. case_bool_decide; wp_pures; [ | case_bool_decide ]; wp_pures.
-      + wp_select. wp_send with "[//]".
-        wp_pures. by iApply "HΦ".
-      + wp_select. wp_send with "[//]".
+    - wp_recv (id') as (Hin') "Hauth".
+      iDestruct (mnat_own_lb_valid with "Hauth Hown") as %[_ Hle'].
+      wp_pures. case_bool_decide as Hdec;
+                  wp_pures; [ | case_bool_decide as Hdec' ]; wp_pures.
+      + wp_select=> /=.
+        iMod (mnat_update_with_lb _ _ id' with "Hauth") as "[Hauth Hown']"=> //.
+        wp_send with "[$Hauth//]".
         wp_pures.
-        replace (id `max` id')%Z with id' by lia.
-        iApply ("IH" with "[Hcl] [Hcr]").
-        { admit. }
-        { admit. }
-        iApply "HΦ".
-      + wp_select. wp_send with "[//]".
-        wp_pures.
-        replace (id `max` id')%Z with id by lia.
-        iApply ("IH" with "[Hcl] [Hcr]").
-        { admit. }
-        { admit. }
-        iApply "HΦ".
-    - wp_pures. wp_select.
-      wp_pures.
-      wp_recv as "_".
-      wp_send with "[//]".
-      wp_pures. by iApply "HΦ".
+        iApply ("IH" $!id' id' with "[] Hown' Hcl Hcr")=> //.
+        iPureIntro. lia.
+      + wp_select. simpl.
+        assert (id = id') as Heq.
+        { inversion Hdec'. lia. }
+        rewrite -Heq.
+        assert (max_out = id) as -> by lia.
+        iDestruct "Hauth" as "[Hauth1 Hauth2]".
+        wp_send with "[$Hauth1//]".
+        wp_pures. iApply "HΦ". eauto.
+      + assert (id ≠ id').
+        { intros Heq. apply Hdec'. by rewrite Heq. }
+        lia.                    (* Contradiction *)
+    - wp_recv (q) as (Hin') "Hauth".
+      wp_select=> /=.
+      iDestruct (mnat_own_lb_valid with "Hauth Hown") as %[_ Hle'].
+      assert (id < max_in) as Hle'' by admit. (* max_in always largest here *)
+      assert (max_in = max_out) as -> by lia.
+      iDestruct "Hauth" as "[Hauth1 Hauth2]".
+      wp_send with "[$Hauth1//]".
+      wp_pures. iApply "HΦ". eauto with lia.
   Admitted.
+
+  Lemma preprocess_spec γ ids (id:nat) cl cr :
+    id ∈ ids →
+    {{{ cl ↣ rle_preprot γ ids ∗ cr ↣ iProto_dual (rle_preprot γ ids) }}}
+      process #id cl cr
+    {{{ res q, RET #res; ⌜id <= res⌝ ∗ ⌜res ∈ ids⌝ ∗ mnat_own_auth γ q res }}}.
+  Proof.
+    iIntros (Hin Φ) "(Hcl & Hcr) HΦ".
+    wp_rec.
+    wp_recv as "_".
+    wp_recv (id') as (Hin') "Hauth".
+    wp_pures.
+    case_bool_decide as Hdec; wp_pures; [ | case_bool_decide as Hdec' ]; wp_pures.
+    + wp_send with "[//]".
+      iMod (mnat_update_with_lb _ _ id' with "Hauth") as "[Hauth Hown]"=> //.
+      wp_send with "[$Hauth//]".
+      wp_apply (process_spec with "[$Hown $Hcl $Hcr]");
+        [ done | iPureIntro; lia |].
+      by iApply "HΦ".
+    + admit.                    (* Not possible in first iteration *)
+    + wp_send with "[//]".
+      iMod (mnat_update_with_lb _ _ id with "Hauth") as "[Hauth Hown]"=> //.
+      { lia. }
+      wp_send (id) with "[$Hauth//]".
+      wp_apply (process_spec with "[$Hown $Hcl $Hcr]");
+        [ done | iPureIntro; lia |].
+      by iApply "HΦ".
+  Admitted.
+
+  Lemma process_start_spec γ ids (id:nat) cl cr :
+    id ∈ ids →
+    {{{ mnat_own_lb γ id ∗
+        cl ↣ rle_prot γ ids id ∗ cr ↣ iProto_dual (rle_preprot γ ids) }}}
+      process #id cl cr
+    {{{ res q, RET #res; ⌜id <= res⌝ ∗ ⌜res ∈ ids⌝ ∗ mnat_own_auth γ q res }}}.
+  Proof.
+    iIntros (Hin Φ) "(Hown & Hcl & Hcr) HΦ".
+    wp_rec.
+    wp_recv as "_".
+    wp_recv (id') as (Hin') "Hauth".
+    wp_pures.
+    case_bool_decide as Hdec; wp_pures; [ | case_bool_decide as Hdec' ]; wp_pures.
+    + wp_select.
+      iMod (mnat_update_with_lb _ _ id' with "Hauth") as "[Hauth Hown']"=> //.
+      wp_send with "[$Hauth//]".
+      wp_apply (process_spec with "[$Hown' $Hcl $Hcr]");
+        [ done | iPureIntro; lia |].
+      by iApply "HΦ".
+    + wp_select. simpl.
+      assert (id = id') as Heq.
+      { inversion Hdec'. lia. }
+      rewrite -Heq.
+      iDestruct "Hauth" as "[Hauth1 Hauth2]".
+      wp_send with "[$Hauth1//]".
+      wp_pures. iApply "HΦ". eauto.
+    + wp_select.
+      iMod (mnat_update_with_lb _ _ id with "Hauth") as "[Hauth Hown']"=> //.
+      { lia. }
+      wp_send (id) with "[$Hauth//]".
+      wp_apply (process_spec with "[$Hown' $Hcl $Hcr]");
+        [ done | iPureIntro; lia |].
+      by iApply "HΦ".
+  Qed.
+
+  Lemma program_spec :
+    {{{ True }}} program #() {{{ RET #3; True }}}.
+  Proof.
+    iIntros (Φ) "_ HΦ".
+    wp_lam.
+    iMod (mnat_alloc 1) as (γ) "[Hauth Hown]".
+    set (ids:={[1 ; 2 ; 3]}:gset nat).
+    wp_apply (new_chan_spec (rle_preprot γ ids))=> //.
+    iIntros (c1l c1r) "[Hc1l Hc1r]".
+    wp_apply (new_chan_spec (rle_preprot γ ids))=> //.
+    iIntros (c2l c2r) "[Hc2l Hc2r]".
+    wp_apply (new_chan_spec (rle_preprot γ ids))=> //.
+    iIntros (c3l c3r) "[Hc3l Hc3r]".
+    wp_send with "[//]".
+    wp_send (1) with "[$Hauth//]".
+    wp_pures.
+    wp_apply (par_spec
+      (λ v, ∃ (res1:nat) q1, ⌜v = #res1⌝ ∗ ⌜1 ≤ res1⌝ ∗ ⌜res1 ∈ ids⌝ ∗
+                             mnat_own_auth γ q1 res1)%I
+      (λ v, ∃ (res2 res3:nat) q2 q3, ⌜v = PairV #res2 #res3⌝ ∗
+                                     ⌜2 ≤ res2⌝ ∗ ⌜res2 ∈ ids⌝ ∗
+                                     ⌜3 ≤ res3⌝ ∗ ⌜res3 ∈ ids⌝ ∗
+                                     mnat_own_auth γ q2 res2 ∗
+                                     mnat_own_auth γ q3 res3 )%I
+                with "[Hown Hc1l Hc3r] [-HΦ]").
+    { wp_apply (process_start_spec γ ids 1 with "[$Hown $Hc1l $Hc3r]");
+        [ set_solver | eauto ]. }
+    { wp_apply (par_spec
+        (λ v, ∃ (res2:nat) q2, ⌜v = #res2⌝ ∗ ⌜2 ≤ res2⌝ ∗ ⌜res2 ∈ ids⌝ ∗
+                               mnat_own_auth γ q2 res2)%I
+        (λ v, ∃ (res3:nat) q3, ⌜v = #res3⌝ ∗ ⌜3 ≤ res3⌝ ∗ ⌜res3 ∈ ids⌝ ∗
+                               mnat_own_auth γ q3 res3)%I
+                  with "[Hc2l Hc1r] [Hc3l Hc2r]").
+      { wp_apply (preprocess_spec γ ids 2 with "[$Hc2l $Hc1r]");
+          [ set_solver | eauto ]. }
+      { wp_apply (preprocess_spec γ ids 3 with "[$Hc3l $Hc2r]");
+          [ set_solver | eauto]. }
+      iIntros (v1 v2) "[H1 H2]".
+      iDestruct "H1" as (res2 q2 -> Hle2 Hin2) "Hauth1".
+      iDestruct "H2" as (res3 q3 -> Hle3 Hin3) "Hauth2".
+      iIntros "!>". iExists res2, res3, q2, q3. eauto with iFrame. }
+    iIntros (v1 v2) "[H1 H2]".
+    iDestruct "H1" as (res1 q1 -> Hle1 Hin1) "Hauth1".
+    iDestruct "H2" as (res2 res3 q2 q3 -> Hle2 Hin2 Hle3 Hin3) "[Hauth2 Hauth3]".
+    iDestruct (mnat_own_auth_agree with "Hauth1 Hauth2") as %[_ <-].
+    iDestruct (mnat_own_auth_agree with "Hauth2 Hauth3") as %[_ <-].
+    iIntros "!>". wp_pures.
+    wp_apply wp_assert. wp_pures. iSplitR; [ by case_bool_decide | ].
+    iIntros "!>".
+    wp_apply wp_assert. wp_pures. iSplitR; [ by case_bool_decide | ].
+    iIntros "!>". wp_pures.
+    assert (res1 = 3) as ->.
+    { set_solver by auto with lia. }
+    by iApply "HΦ".
+  Qed.
 
 End ring_leader_election_example.
